cp

steel/Veritas.Steel.PRFSetHash.fsti
@@ -6,6 +6,7 @@ open Steel.Effect
 open Steel.Reference
 open Steel.Array
 open FStar.Ghost
+module U8 = FStar.UInt8
 module U16 = FStar.UInt16
 module U32 = FStar.UInt32
 module U64 = FStar.UInt64
@@ -14,21 +15,27 @@ module T = Veritas.Formats.Types
 open Veritas.Steel.VerifierModel
 open Veritas.ThreadStateModel
 module AT = Steel.Effect.Atomic
-val prf_set_hash : Type0
+module VFT = Veritas.Formats.Types
+module MSH = Veritas.MultiSetHash
+module A = Veritas.Steel.Array
+module HA = Veritas.Steel.HashAccumulator
 
-// AF: Internally, should probably be implemented with a ghost reference to the model_hash
-// The selector would then fetch the value in the ghost state
-// The reason why we would need a ghost state is that the "spec" contains strictly more
-// information than the concrete value. So we cannot reconstruct it out of just the concrete state
-val prf_set_hash_sl (_:prf_set_hash) : slprop u#1
-val prf_set_hash_sel (r:prf_set_hash) : selector (model_hash) (prf_set_hash_sl r)
+val prf_set_hash
+  : Type0
+
+val prf_set_hash_sl (_:prf_set_hash)
+  : slprop u#1
+
+val prf_set_hash_sel (r:prf_set_hash)
+  : selector (HA.hash_value_t) (prf_set_hash_sl r)
 
 [@@__steel_reduce__]
 noextract
-let prf_set_hash_inv' (r:prf_set_hash) : vprop' =
-  { hp = prf_set_hash_sl r;
-    t = model_hash;
-    sel = prf_set_hash_sel r}
+let prf_set_hash_inv' (r:prf_set_hash)
+  : vprop'
+  = { hp = prf_set_hash_sl r;
+      t = HA.hash_value_t;
+      sel = prf_set_hash_sel r}
 
 unfold
 let prf_set_hash_inv (r:prf_set_hash)
@@ -38,8 +45,9 @@ let prf_set_hash_inv (r:prf_set_hash)
 [@@ __steel_reduce__]
 let v_hash (#p:vprop)
            (r:prf_set_hash)
-           (h:rmem p{FStar.Tactics.with_tactic selector_tactic (can_be_split p (prf_set_hash_inv r) /\ True)})
-  : GTot model_hash
+           (h:rmem p{FStar.Tactics.with_tactic selector_tactic
+                      (can_be_split p (prf_set_hash_inv r) /\ True)})
+  : GTot HA.hash_value_t
   = h (prf_set_hash_inv r)
 
 val create (_:unit)
@@ -47,49 +55,50 @@ val create (_:unit)
     emp
     (fun p -> prf_set_hash_inv p)
     (requires fun _ -> True)
-    (ensures fun _ p h1 -> v_hash p h1 == init_hash)
+    (ensures fun _ p h1 -> v_hash p h1 == HA.initial_hash)
 
 val free (p:prf_set_hash)
   : SteelT unit
     (prf_set_hash_inv p)
     (fun _ -> emp)
 
-module VFT = Veritas.Formats.Types
+val update_hash_value (ha:HA.hash_value_t)
+                      (r:T.record)
+                      (t:T.timestamp)
+                      (thread_id:T.thread_id)
+  : GTot HA.hash_value_t
 
-val prf_update_hash (p:prf_set_hash) (r:T.record) (t:T.timestamp) (thread_id:T.thread_id)
+val prf_update_hash (p:prf_set_hash)
+                    (r:T.record)
+                    (t:T.timestamp)
+                    (thread_id:T.thread_id)
   : Steel unit
     (prf_set_hash_inv p)
     (fun _ -> prf_set_hash_inv p)
     (requires fun _ -> True)
-    (ensures fun h0 _ h1 -> v_hash p h1 == model_update_hash (v_hash p h0) r t thread_id)
+    (ensures fun h0 _ h1 ->
+      v_hash p h1 == update_hash_value (v_hash p h0) r t thread_id)
 
-module A = Steel.Array
-module U8 = FStar.UInt8
-
-val as_model_hash (s:Seq.lseq U64.t 4) : model_hash
-val prf_read_hash (p:prf_set_hash) (out:A.array U64.t)
+val prf_read_hash (p:prf_set_hash) (out:A.array U8.t)
   : Steel unit
     (prf_set_hash_inv p `star` A.varray out)
     (fun _ -> prf_set_hash_inv p `star` A.varray out)
-    (requires fun _ -> A.length out == 4)
+    (requires fun _ -> A.length out == 32)
     (ensures fun h0 _ h1 ->
-      A.length out == 4 /\
+      A.length out == 32 /\
       v_hash p h0 == v_hash p h1 /\
-      as_model_hash (A.asel out h1) == v_hash p h1)
+      A.asel out h1 == v_hash p h1)
 
-module MSH = Veritas.MultiSetHash
-val prf_hash_agg (a0 a1:A.array U64.t)
+val prf_hash_agg (a0 a1:A.array U8.t)
   : Steel unit
     (A.varray a0 `star` A.varray a1)
     (fun _ -> A.varray a0 `star` A.varray a1)
     (requires fun _ ->
-      A.length a0 == 4 /\
-      A.length a1 == 4)
+      A.length a0 == 32 /\
+      A.length a1 == 32)
     (ensures fun h0 _ h1 ->
-      A.length a0 == 4 /\
-      A.length a1 == 4 /\
-      as_model_hash (A.asel a1 h0) ==
-         as_model_hash (A.asel a1 h1) /\
-      as_model_hash (A.asel a0 h1) ==
-        MSH.ms_hashfn_agg (as_model_hash (A.asel a0 h0))
-                          (as_model_hash (A.asel a1 h0)))
+      A.length a0 == 32 /\
+      A.length a1 == 32 /\
+      A.asel a1 h0 == A.asel a1 h1 /\
+      A.asel a0 h1 ==
+        HA.aggregate_hash_value (A.asel a0 h0) (A.asel a1 h0))
