steel/Veritas.Steel.PRFSetHash.fst
@@ -1,0 +1,123 @@
+module Veritas.Steel.PRFSetHash
+
+open Steel.Memory
+open Steel.Effect.Atomic
+open Steel.Effect
+open Steel.Reference
+open Steel.Array
+open FStar.Ghost
+module U16 = FStar.UInt16
+module U32 = FStar.UInt32
+module U64 = FStar.UInt64
+
+module T = Veritas.Formats.Types
+open Veritas.Steel.VerifierModel
+open Veritas.ThreadStateModel
+module AT = Steel.Effect.Atomic
+module VFT = Veritas.Formats.Types
+module VF = Veritas.Formats
+module MSH = Veritas.MultiSetHash
+module HA = Veritas.Steel.HashAccumulator
+
+let prf_set_hash = HA.state
+
+let prf_set_hash_sl (s:prf_set_hash)
+  : slprop u#1
+  = A.is_array s
+
+let prf_set_hash_sel (r:prf_set_hash)
+  : selector (HA.hash_value_t) (prf_set_hash_sl r)
+  = A.array_sel r
+
+let create () =
+  let x = HA.create_in () in
+  AT.change_equal_slprop (A.varray _)
+                         (prf_set_hash_inv _);
+  AT.return x
+
+let free (p:prf_set_hash)
+  = AT.change_equal_slprop (prf_set_hash_inv _)
+                           (A.varray _);
+    HA.free p
+
+let update_hash_value (ha:HA.hash_value_t)
+                      (r:T.record)
+                      (t:T.timestamp)
+                      (tid:T.thread_id)
+  : GTot HA.hash_value_t
+  = let b = VF.serialize_stamped_record_spec (VFT.({ sr_record = r; sr_timestamp = t; sr_thread_id = tid})) in
+    let h = HA.hash_value b in
+    HA.aggregate_hash_value ha h
+
+#push-options "--query_stats"
+let prf_update_hash' (p:prf_set_hash)
+                     (r:T.record)
+                     (t:T.timestamp)
+                     (tid:T.thread_id)
+  : Steel unit
+    (A.varray p)
+    (fun _ -> A.varray p)
+    (requires fun _ -> True)
+    (ensures fun h0 _ h1 ->
+      A.asel p h1 == update_hash_value (A.asel p h0) r t tid)
+  =  let h0 = AT.get () in
+     let sr = (VFT.({ sr_record = r; sr_timestamp = t; sr_thread_id = tid})) in
+     let tmp = A.malloc 0uy 184ul in
+     let len = VF.serialize_stamped_record tmp sr in
+     let h1 = AT.get () in
+     HA.add p tmp len;
+     A.free tmp;
+     AT.slassert (A.varray p);
+     let h2 = AT.get () in
+     assert (A.asel p h2 ==
+             HA.aggregate_hash_value (A.asel p h1)
+                                     (HA.hash_value
+                                       (Seq.slice (A.asel tmp h1) 0 (U32.v len))));
+     assert (Seq.slice (A.asel tmp h1) 0 (U32.v len) ==
+             VF.serialize_stamped_record_spec sr);
+     assert (A.asel p h2 ==
+             HA.aggregate_hash_value
+               (A.asel p h1)
+               (HA.hash_value (VF.serialize_stamped_record_spec sr)));
+     assert_spinoff (A.asel p h2 ==
+                     update_hash_value (A.asel p h1) r t tid)
+
+let prf_update_hash p r t tid =
+  AT.change_equal_slprop (prf_set_hash_inv p)
+                         (A.varray p);
+  prf_update_hash' p r t tid;
+  AT.change_equal_slprop (A.varray p)
+                         (prf_set_hash_inv p)
+
+let prf_read_hash' (p:prf_set_hash) (out:A.array U8.t)
+  : Steel unit
+    (A.varray p `star` A.varray out)
+    (fun _ -> A.varray p `star` A.varray out)
+    (requires fun _ -> A.length out == 32)
+    (ensures fun h0 _ h1 ->
+      A.length out == 32 /\
+      A.asel p h0 == A.asel p h1 /\
+      A.asel out h1 == A.asel p h1)
+  = HA.get p out
+
+let prf_read_hash (p:prf_set_hash) (out:A.array U8.t)
+  = AT.change_equal_slprop (prf_set_hash_inv p)
+                           (A.varray p);
+    prf_read_hash' p out;
+    AT.change_equal_slprop (A.varray p)
+                           (prf_set_hash_inv p)
+
+let prf_hash_agg (a0 a1:A.array U8.t)
+  : Steel unit
+    (A.varray a0 `star` A.varray a1)
+    (fun _ -> A.varray a0 `star` A.varray a1)
+    (requires fun _ ->
+      A.length a0 == 32 /\
+      A.length a1 == 32)
+    (ensures fun h0 _ h1 ->
+      A.length a0 == 32 /\
+      A.length a1 == 32 /\
+      A.asel a1 h0 == A.asel a1 h1 /\
+      A.asel a0 h1 ==
+        HA.aggregate_hash_value (A.asel a0 h0) (A.asel a1 h0))
+  = HA.aggregate_hash_value_buf a0 a1
